
DC (1991, Biham)
LC (1993, Matsui)

- Linear Cryptanalysis: KPA
- Linear Approximation

DC; $\Delta x=\alpha, \Delta y=\beta$; $p[\alpha\to\beta]=p\gg 1/2^n$

LC; $a$: input mask / $\beta$: output mask; for $x_i,y_i\in GF(2)$
$$
a\cdot x=b\cdot y\iff \bigoplus_{i=1}^na_ix_i=\bigoplus_{i=1}^nb_iy_i
$$
-> 1-bit relation (1/2)

> [!note] Linear Function
> - Linear and Non-linear ($f:\mathbb{R}\to\mathbb{R}$)
> $$
> f(x+y)=f(x)+f(y), f(ax)=af(x)
> $$
> - Boolean Ftn ($f:\set{0,1}\to \set{0,1}$)
> $$
> f(x\oplus y)=f(x)\oplus f(y), f(ax)=af(x)
> - Multi-variable Boolean Ftn ($f:\set{0,1}^n\to\set{0,1}$)
> $$
> f(x)=a\cdot x=\bigoplus_{i=1}^n a_ix_i
> $$
> - Vector Boolean Ftn ($f:\set{0,1}^n\to\set{0,1}^m$)
> $$
> f(x)=Ax, A\in M_{m\times n}(\mathbb{F}_2)

> [!note] Linearity
> - $x\in\set{0,1}^n,y\in\set{0,1}^m$;
> $$
> a\cdot x=b\cdot y\iff \bigoplus_{i=1}^na_ix_i=\bigoplus_{i=1}^nb_iy_i
> $$
> - $y=Ax$;
> $$
> \begin{bmatrix}
> y_0\\ y_1 \\ y_2\\ y_3
> \end{bmatrix}=
> \begin{bmatrix}
> a_{00} & a_{01} & a_{02} & a_{03} \\
> a_{10} & a_{11} & a_{12} & a_{13} \\
> a_{20} & a_{21} & a_{22} & a_{23} \\
> a_{30} & a_{31} & a_{32} & a_{33} \\
> \end{bmatrix}
> \begin{bmatrix}
> x_0\\ x_1 \\ x_2\\ x_3
> \end{bmatrix}
> $$
> $y_i=\bigoplus_{j=0}^n a_{ij}x_j$


> [!note] Linear Approximation Probability
> 1. For boolean ftn $S:\set{0,1}^n\to\set{0,1}^m$,
> - Number $NS(a,b):=\#\set{x\in\mathbb{F}_2^n : a\cdot x=b\cdot S(x)\in\mathbb{F}_2}$
> - Distribution $\lambda_S(a,b)=NS(a,b)-2^{n-1}$
> 
> 2. Linear Hull Probability
> 
> 3. Linear Approximation Probability
> $$
> \frac{NS(a,b)}{2^n}
> $$

> [!example] 3-bit boolean function $S$
> - S[8] = {0, 1, 7, 2, 3, 4, 5, 6}
> - $a=001$, $b=011$
> 

| $x$ | $a\cdot x$ | $y=S(x)$ | $b\cdot y$ | $a\cdot x=b\cdot y$ |
| --- | ---------- | -------- | ---------- | ------------------- |
| 000 | 0          | 000      | 0          | O                   |
| 001 | 1          | 001      | 1          | O                   |
| 010 | 0          | 111      | 0          | O                   |
| 011 | 1          | 010      | 1          | O                   |
| 100 | 0          | 011      | 0          | O                   |
| 101 | 1          | 100      | 0          | X                   |
| 110 | 0          | 101      | 1          | X                   |
| 111 | 1          | 110      | 1          | O                   |

 -> probability: $6/8=3/4$


> [!example] CipherWC8
> - $u,v,w,z$
> 	- $u=m\oplus k_0$
> 	- $v=S(u)$
> 	- $w=S^{-1}(z)$
> 	- $z=c\oplus k_2$
> - Linear Cryptanalysis for 2R
> 	1) Guess $k_2\in\set{0,1,\dots,255}$
> 	2) Compute $w=S^{-1}(z)=S^{-1}(c\oplus k_2)$
> 	3) If $k_2$ is correct, it satisfies $a\cdot u=b\cdot u$:
> 	   $$
> 	   a\cdot(m\oplus k_0)=b\cdot(S^{-1}(c\oplus k_2)\oplus k_1)\quad\cdots\cdots(*)
> 	   $$
> 	4) Rearrange ( * ):
> 	   $$
> 	   (a\cdot m)\oplus(a\cdot k_0)\oplus b\cdot S^{-1}(c\oplus k_2)\oplus (b\cdot k_1)=0
> 	   $$
> 	   $$
> 	   a\cdot m\oplus b\cdot S^{-1}(c\oplus k_2)=a\cdot k_0\oplus b\cdot k_1
> 	   $$
> 	   For (PT,CT) pairs: $(m_1,c_1),\dots,(m_n,c_n)$,
> 	   $$
> 	   \begin{align*}
> 	   (m_1,c_1) &\implies am_1\oplus bS^{-1}(c_1\oplus k_2)=ak_0\oplus bk_1\\
> 	   &\vdots\\
> 	   (m_n,c_n) &\implies am_n\oplus bS^{-1}(c_n\oplus k_2)=ak_0\oplus bk_1\\
> 	   \end{align*}
> 	   $$
> 	   Here, $ak_0\oplus bk_1\in\set{0,1}$ is fixed
> 	5) If $k_2$ is correct, LHS is constant with probability $p$
> 	   else LHS=RHS with probability $1/2$
> 	6) Determinant
> 	   $$
> 	   am\oplus bS^{-1}(c\oplus k_2)=ak_0\oplus bk_1 (=Constant)
> 	   $$


> [!theorem] Piling-up Lemma
> Let $X_1,\dots, X_n\in\mathbb{F}_2$ are independent random variables. Let $P(X_i=0)=1/2+\epsilon_i$, $|\epsilon_i|\leq1/2$. Then
> $$
> P(X_1\oplus X_2\oplus \cdots\oplus X_n=0)=1/2+2^{n-1}\epsilon_1\epsilon_2\cdots\epsilon_n
> $$

| $X_i$    | 0                | 1                |
| -------- | ---------------- | ---------------- |
| $P(X_i)$ | $1/2+\epsilon_i$ | $1/2-\epsilon_i$ |


> [!example]
> - $ax=bS(x)$ with $p_1$
> - $cx=dS(x)$ with $p_2$
> - $u,v,w,z,y,x$
> 	- $u=m\oplus k_0$
> 	- $z=y\oplus k_2=S^{-1}(c\oplus k_2)\oplus k_2$
> 
> Formula 1 $\cdots\cdots P(au\oplus bu=0)=p_1$
> Formula 2 $\cdots\cdots P(bw\oplus dz=0)=p_2$
> $P(au\oplus bu\oplus bw\oplus dz=0)=p=p_1p_2+(1-p_1)(1-p_2)$
> 
> Determinant:
> $$
> a(m\oplus k_0)\oplus b(v\oplus w)\oplus d(S^{-1}(c\oplus k_3)\oplus k_2)=0
> $$
> $$
> \Leftrightarrow am\oplus dS^{-1}(c\oplus k_3)=ak_0\oplus bk_1\oplus dk_2\quad\text{with}\ p
> $$









