
---
> [!info] **Observation**
> Let
> - $R=\mathbb{Z}$
> - $S = \mathbb{Z}^*=\mathbb{Z}\setminus \set{0}$
> 
> Then $$
> S^{-1}R=(\mathbb{Z}^*)^{-1}\mathbb{Z}=\left\{ \frac{n}{m}:n\in\mathbb{Z},\ m\in\mathbb{Z}^* \right\}=\mathbb{Q}.
> $$


> [!abstract] **Definition**
> A graph is defined as...


> [!important] **Theorem**
> Let $f$ be continuous...

> [!check] **Proof**
> By induction...

> [!example] **Example**
> Let
> - $R=\mathbb{C}[x]$
> - $S = \{1,(x-1),(x-1)^2,\dots\}=\{ (x-1)^n:n\in\mathbb{Z}_{{\geq 0}} \}$
> 
> Then 
> $$
> S^{-1}R=\left\{ \frac{f(x)}{(x-1)^n}:f\in\mathbb{C}[x],\ n\in\mathbb{Z}_{{\geq {0}}} \right\}.
> $$
> This localization "inverts" the powers of $(x−1)$, meaning that (x−1) becomes a unit in the localized ring $S^{-1}R$.





> [!note] **Notes**
> In further exploration...



